case_studies/cp/README.md
@@ -1,3 +1,3 @@
 # CP
 
-This directory contains a mechanization of the session-typed process calculus CP, with a proof of cut elimination / progress.
+This subdirectory contains a mechanization of (a fragment of) the session-typed process calculus CP, with a proof of cut elimination / progress.
